VsaIris.lean
@@ -142,6 +142,7 @@ import VsaIris.Vsa.SnpMove
 import VsaIris.Vsa.SnpPuts
 import VsaIris.Vsa.SnpPrint
 import VsaIris.Vsa.SnpStrlen
+import VsaIris.Vsa.SnpSvf
 import VsaIris.Interp.IRun
 import VsaIris.Interp.Steps
 import VsaIris.Interp.ITac
